feat: finish exercise10 and 11

Exercise10.dfy
@@ -1,15 +1,250 @@
+// Exercise10.1
 class UniqueNumberAllocator {
   ghost var used: set<nat>
-  ghost predicate Valid( )
+  var next: nat
+
+  ghost predicate Valid()
     reads this
-  constructor ( )
-    ensures Valid( ) && used == {}
-  method Allocate( ) returns (n: nat)
-    requires Valid( )
+  {
+    // built relation between next and used: used = {0, 1, 2, ..., next - 1}
+    forall n :: 0 <= n < next <==> n in used
+  }
+  constructor ()
+    ensures Valid() && used == {}
+  {
+    //Initialize the allocator
+    next := 0;
+    used := {};
+  }
+
+  method Allocate() returns (n: nat)
+    requires Valid()
     modifies this
-    ensures Valid( ) && n !in old(used) && used == old(used) + {n}
-  method Reset( )
-    requires Valid( )
+    ensures Valid() && n !in old(used) && used == old(used) + {n}
+  {
+    n := next;
+    next := next + 1;
+    used := used + {n};
+  }
+
+  method Reset()
+    requires Valid()
     modifies this
-    ensures Valid( ) && used == {}
+    ensures Valid() && used == {}
+  {
+    next := 0;
+    used := {};
+  }
+}
+
+// Exercise10.2
+class Grinder {
+  ghost var hasBeans: bool
+  ghost var Repr: set<object>
+
+  ghost predicate Valid()
+    reads this, Repr
+    ensures Valid() ==> this in Repr
+
+  constructor()
+    ensures Valid() && fresh(Repr) && !hasBeans
+
+  function Ready(): bool
+    requires Valid()
+    reads Repr
+    ensures Ready() == hasBeans
+
+  method AddBeans()
+    requires Valid()
+    modifies Repr
+    ensures Valid() && hasBeans && fresh(Repr-old(Repr))
+
+  method Grind()
+    requires Valid() && hasBeans
+    modifies Repr
+    ensures Valid() && fresh(Repr-old(Repr))
+}
+
+class WaterTank {
+  ghost var waterLevel: nat
+  ghost var Repr: set<object>
+
+  ghost predicate Valid()
+    reads this, Repr
+    ensures Valid() ==> this in Repr
+
+  constructor()
+    ensures Valid() && fresh(Repr) && waterLevel == 0
+
+  function Level(): nat
+    requires Valid()
+    reads Repr
+    ensures Level() == waterLevel
+
+  method Fill()
+    requires Valid()
+    modifies Repr
+    ensures Valid() && fresh(Repr-old(Repr)) && waterLevel == 10
+
+  method Use()
+    requires Valid() && waterLevel != 0
+    modifies Repr
+    ensures Valid() && fresh(Repr-old(Repr)) && waterLevel == old(waterLevel) - 1
+}
+
+class CoffeeMaker {
+  ghost var ready: bool
+  ghost var Repr: set<object>
+  var g: Grinder
+  var w: WaterTank
+
+  ghost predicate Valid()
+    reads this, Repr
+    ensures Valid() ==> this in Repr
+  {
+    this in Repr && g in Repr && w in Repr &&
+    g.Repr <= Repr && w.Repr <= Repr &&
+    w.Repr !! g.Repr !! {this} &&
+    g.Valid() && w.Valid() &&
+    ready == (g.hasBeans && w.waterLevel != 0)
+  }
+
+  constructor()
+    ensures Valid() && fresh(Repr)
+  {
+    g := new Grinder();
+    w := new WaterTank();
+    ready := false;
+    new;
+    Repr := {this, g, w} + g.Repr + w.Repr;
+  }
+
+  predicate Ready()
+    requires Valid()
+    reads Repr
+    ensures Ready() == ready
+  {
+    g.Ready() && w.Level() != 0
+  }
+
+  method Restock()
+    requires Valid()
+    modifies Repr
+    ensures Valid() && Ready() && fresh(Repr - old(Repr))
+  {
+    assert w.Valid();
+    assert w.Repr !! g.Repr;
+    assert this !in g.Repr;
+    g.AddBeans();
+    assert w.Valid();
+    w.Fill();
+    ready := true;
+    Repr := Repr + g.Repr + w.Repr;
+  }
+
+  method Dispense()
+    requires Valid() && Ready() && w.waterLevel != 0
+    modifies Repr
+    ensures Valid() && fresh(Repr - old(Repr))
+  {
+    g.Grind();
+    w.Use();
+    ready := g.hasBeans && w.waterLevel != 0;
+    Repr := Repr + g.Repr + w.Repr;
+  }
+
+  method ChangeGrinder()
+    requires Valid()
+    modifies Repr
+    ensures Valid() && fresh(Repr - old(Repr))
+  {
+    g := new Grinder();
+    ready := false;
+    Repr := Repr + g.Repr;
+  }
+
+  method InstallCustomGrinder(grinder: Grinder)
+    requires Valid() && grinder.Valid() && grinder.Repr !! Repr
+    modifies Repr
+    ensures Valid() && fresh(Repr - old(Repr) - grinder.Repr)
+  {
+    g := grinder;
+    ready := (g.hasBeans && w.waterLevel > 0);
+    Repr := Repr + g.Repr;
+  }
+}
+
+method TestHarness() {
+  var cm := new CoffeeMaker();
+  cm.Restock();
+  assert cm.Ready();
+  cm.Dispense();
+}
+
+// Exercise10.3
+class BoundedQueue<T(0)> {
+  ghost var contents: seq<T>
+  ghost var N: nat
+  ghost var Repr: set<object>
+  var data: array<T>
+  var wr: nat
+  var rd: nat
+  var empty: bool
+
+  ghost predicate Valid()
+    reads this, Repr
+    ensures Valid() ==> this in Repr && |contents| <= N
+  {
+    this in Repr && data in Repr &&
+    0 < data.Length == N && wr < N && rd < N &&
+    (empty ==> rd == wr) &&
+    contents == if rd < wr then data[rd..wr] else if !empty then data[rd..] + data[..wr] else [ ]
+  }
+
+  constructor (N: nat)
+    requires N > 0
+    ensures Valid() && fresh(Repr) && contents == [] && this.N == N
+  {
+    contents := [];
+    this.N := N;
+    data := new T[N];
+    rd, wr, empty := 0, 0, true;
+    Repr := {this, data};
+  }
+
+  method Insert(x: T)
+    requires Valid()
+    requires |contents| != N
+    modifies Repr
+    ensures contents == old(contents) + [x]
+    ensures N == old(N)
+    ensures Valid() && fresh(Repr - old(Repr))
+  {
+    contents := contents + [x];
+    data[wr] := x;
+    if wr == data.Length - 1 {
+      wr := 0;
+    } else {
+      wr := wr + 1;
+    }
+    empty := false;
+  }
+
+  method Remove() returns (x: T)
+    requires Valid()
+    requires |contents| != 0
+    modifies Repr
+    ensures contents == old(contents[1..]) && x == old(contents[0])
+    ensures N ==old(N)
+    ensures Valid() && fresh(Repr - old(Repr))
+  {
+    contents := contents[1..];
+    x := data[rd];
+    if rd == data.Length - 1 {
+      rd := 0;
+    } else {
+      rd := rd + 1;
+    }
+    empty := (rd == wr);
+  }
 }
