Exercise11.dfy
@@ -1,0 +1,96 @@
+class Stack<T> {
+  ghost var s: seq<T>
+  ghost var Repr: set<object>
+  var top: Node?<T>
+
+  ghost predicate Valid()
+    reads this, Repr
+    ensures Valid() ==> this in Repr
+  {
+    this in Repr &&
+    (top == null ==> s == []) &&
+    (top != null ==> top in Repr && top.Repr <= Repr && this !in top.Repr &&
+                     top.Valid() && top.s == s)
+  }
+
+  constructor()
+    ensures Valid() && fresh(Repr)
+    ensures s == []
+  {
+    top := null;
+    s, Repr := [], {this};
+  }
+
+  method Push(v: T)
+    requires Valid()
+    modifies Repr
+    ensures Valid() && fresh(Repr - old(Repr))
+    ensures s == [v] + old(s)
+  {
+    var newNode := new Node(v);
+    if top != null {
+      newNode.SetNext(top);
+    }
+    top := newNode;
+    s, Repr := [v] + s, {this} + newNode.Repr;
+  }
+  method Pop() returns (v: T)
+    requires s != []
+    requires Valid()
+    modifies Repr
+    ensures Valid() && fresh(Repr - old(Repr))
+    ensures v == old(s[0]) && s == old(s[1..])
+  {
+    v := top.GetValue();
+    top := top.GetNext();
+    s := s[1..]; // note that the removal of old(top) from Repr is not required
+  }
+}
+
+class Node<T> {
+  ghost var s: seq<T>
+  ghost var Repr: set<object>
+  var value: T
+  var next: Node?<T>
+
+  ghost predicate Valid()
+    reads this, Repr
+    ensures Valid() ==> this in Repr && |s| > 0
+  {
+    this in Repr &&
+    (next == null ==> s == [value]) &&
+    (next != null ==> next in Repr && next.Repr <= Repr && this !in next.Repr &&
+                      next.Valid() && s == [value] + next.s)
+  }
+  constructor (v: T)
+    ensures Valid() && fresh(Repr)
+    ensures s == [v]
+  {
+    value := v;
+    next := null;
+    s, Repr := [v], {this};
+  }
+  method SetNext(n: Node<T>)
+    requires Valid() && n.Valid() && this !in n.Repr && n.Repr !! Repr
+    modifies Repr
+    ensures Valid() && fresh(Repr - old(Repr) - n.Repr)
+    ensures s == old([s[0]]) + n.s
+  {
+    next := n;
+    s, Repr := [value] + n.s, Repr + next.Repr;
+  }
+  method GetNext() returns (n: Node?<T>) // could also be a function
+    requires Valid()
+    ensures n == null ==> |s| == 1
+    ensures n != null ==> n in Repr && n.Repr <= Repr && this !in n.Repr &&
+                          n.Valid() && s == [s[0]] + n.s
+  {
+    n := next;
+  }
+  method GetValue() returns (v: T) // could also be a function
+    requires Valid()
+    ensures v == s[0]
+  {
+    v := value;
+  }
+}
